src/FcEtt/ett_rename.v
@@ -1,0 +1,209 @@
+Require Export FcEtt.imports.
+Require Import ett_ott.
+Require Import ett_inf.
+Require Import ett_match.
+
+Inductive pattern_renamed : tm -> tm -> available_props ->
+                                        available_props -> Prop :=
+ | pattern_renamed_Base : forall (F:const) (D:available_props),
+     pattern_renamed (a_Fam F) (a_Fam F) D  AtomSetImpl.empty
+ | pattern_renamed_AppRel : forall (p1:tm) (R:role) (x:tmvar) (p2:tm)
+                                  (y:tmvar) (D D':available_props),
+     pattern_renamed p1 p2 D D' -> ~ AtomSetImpl.In  y (D  \u  D') ->
+     pattern_renamed (a_App p1 (Role R) (a_Var_f x))
+                     (a_App p2 (Role R) (a_Var_f y)) D  (singleton  y  \u  D')
+ | pattern_renamed_AppIrrel : forall (p1 p2:tm) (D D':available_props),
+     pattern_renamed p1 p2 D D' ->
+     pattern_renamed (a_App p1 (Rho Irrel) a_Bullet)
+                     (a_App p2 (Rho Irrel) a_Bullet) D D'
+ | pattern_renamed_CApp : forall (p1 p2:tm) (D D':available_props),
+     pattern_renamed p1 p2 D D' ->
+     pattern_renamed (a_CApp p1 g_Triv) (a_CApp p2 g_Triv) D D'.
+
+Hint Constructors pattern_renamed.
+
+Fixpoint tm_var_pairs (a p : tm) : list (tm * var) :=
+   match (a,p) with
+ | (a_Fam F, a_Fam F') => []
+ | (a_App a1 (Role R) a2, a_App p1 (Role R') (a_Var_f x)) =>
+                                       tm_var_pairs a1 p1 ++ [(a2,x)]
+ | (a_App a (Rho Irrel) a', a_App p (Rho Irrel) a_Bullet) =>
+                                       tm_var_pairs a p
+ | (a_CApp a g_Triv, a_CApp p g_Triv) => tm_var_pairs a p
+ | (_,_) => []
+   end.
+
+Definition chain_subst a p b := fold_left
+       (fun b' a'x' => tm_subst_tm_tm a'x'.1 a'x'.2 b') (tm_var_pairs a p) b.
+
+Lemma chain_subst_fv : forall a p b, tm_pattern_agree a p ->
+      fv_tm_tm_tm (chain_subst a p b) [<=]
+        (AtomSetImpl.diff (fv_tm_tm_tm b) (fv_tm_tm_tm p)) \u (fv_tm_tm_tm a).
+Proof. intros. induction H; eauto.
+        - pose (P := fv_tm_tm_tm_tm_subst_tm_tm_upper (chain_subst a1 p1 b) a2 x).
+          unfold chain_subst in *. simpl. rewrite fold_left_app. simpl.
+          eapply Subset_trans. eapply P. fsetdec.
+        - unfold chain_subst in *. simpl. fsetdec.
+        - unfold chain_subst in *. simpl. fsetdec.
+Qed.
+
+Lemma Rename_pattern_renamed : forall p b p' b' D D', Rename p b p' b' D D' ->
+      pattern_renamed p p' D D'.
+Proof. intros. induction H; eauto.
+Qed.
+
+Lemma Rename_chain_subst : forall p b p' b' D D', Rename p b p' b' D D' ->
+                           b' = chain_subst p' p b.
+Proof. intros. induction H; simpl; eauto.
+       unfold chain_subst in *. simpl. rewrite fold_left_app. simpl.
+       rewrite <- IHRename. auto.
+Qed.
+
+Lemma chain_subst_Rename : forall p b p' D D', pattern_renamed p p' D D' ->
+      lc_tm b -> Rename p b p' (chain_subst p' p b) D D'.
+Proof. intros. induction H; simpl; eauto. unfold chain_subst in *.
+       simpl. rewrite fold_left_app. simpl. eauto.
+Qed.
+
+Lemma matchsubst_chain_subst : forall a p b, tm_pattern_agree a p ->
+                               matchsubst a p b = chain_subst a p b.
+Proof. intros. induction H; simpl; eauto. unfold chain_subst in *. simpl.
+       rewrite fold_left_app. simpl. rewrite <- IHtm_pattern_agree. auto.
+Qed.
+
+Lemma subst_via : forall a y z,
+      (forall b, y `notin` fv_tm_tm_tm b ->
+      tm_subst_tm_tm a y (tm_subst_tm_tm (a_Var_f y) z b) =
+      tm_subst_tm_tm a z b) /\
+      (forall brs, y `notin` fv_tm_tm_brs brs ->
+      tm_subst_tm_brs a y (tm_subst_tm_brs (a_Var_f y) z brs) =
+      tm_subst_tm_brs a z brs) /\
+      (forall g, y `notin` fv_tm_tm_co g ->
+      tm_subst_tm_co a y (tm_subst_tm_co (a_Var_f y) z g) =
+      tm_subst_tm_co a z g) /\
+      (forall phi, y `notin` fv_tm_tm_constraint phi ->
+      tm_subst_tm_constraint a y (tm_subst_tm_constraint (a_Var_f y) z phi) =
+      tm_subst_tm_constraint a z phi).
+Proof. intros. apply tm_brs_co_constraint_mutind; intros; simpl;
+       try (simpl in H; try simpl in H1; try simpl in H2; f_equal; eauto; fail).
+       destruct (eq_var x z). simpl. rewrite eq_dec_refl. auto.
+       simpl. destruct (eq_var x y). subst. simpl in H. fsetdec. auto.
+Qed.
+
+Lemma subst_via_tm : forall a y z b, y `notin` fv_tm_tm_tm b ->
+      tm_subst_tm_tm a y (tm_subst_tm_tm (a_Var_f y) z b) =
+      tm_subst_tm_tm a z b.
+Proof. intros. eapply subst_via; eauto.
+Qed.
+
+Lemma subst_commute : forall a1 a2 x1 x2, x1 `notin` fv_tm_tm_tm a2 ->
+      x2 `notin` fv_tm_tm_tm a1 -> x1 <> x2 ->
+      (forall b, tm_subst_tm_tm a2 x2 (tm_subst_tm_tm a1 x1 b) =
+      tm_subst_tm_tm a1 x1 (tm_subst_tm_tm a2 x2 b)) /\
+      (forall brs, tm_subst_tm_brs a2 x2 (tm_subst_tm_brs a1 x1 brs) =
+      tm_subst_tm_brs a1 x1 (tm_subst_tm_brs a2 x2 brs)) /\
+      (forall g, tm_subst_tm_co a2 x2 (tm_subst_tm_co a1 x1 g) =
+      tm_subst_tm_co a1 x1 (tm_subst_tm_co a2 x2 g)) /\
+      (forall phi, tm_subst_tm_constraint a2 x2
+       (tm_subst_tm_constraint a1 x1 phi) =
+        tm_subst_tm_constraint a1 x1 (tm_subst_tm_constraint a2 x2 phi)).
+Proof. intros a1 a2 x1 x2 P Q R.
+       apply tm_brs_co_constraint_mutind; intros; simpl; eauto;
+       try (f_equal; eauto; fail).
+       destruct (eq_var x x1). destruct (eq_var x x2). subst. contradiction.
+       subst. simpl. rewrite eq_dec_refl. rewrite tm_subst_tm_tm_fresh_eq; auto.
+       destruct (eq_var x x2). subst. simpl. rewrite eq_dec_refl.
+       rewrite tm_subst_tm_tm_fresh_eq; auto.
+       rewrite tm_subst_tm_tm_fresh_eq; auto.
+       rewrite tm_subst_tm_tm_fresh_eq; auto.
+Qed.
+
+Lemma subst_commute_tm : forall a1 a2 x1 x2 b, x1 `notin` fv_tm_tm_tm a2 ->
+      x2 `notin` fv_tm_tm_tm a1 -> x1 <> x2 ->
+      tm_subst_tm_tm a2 x2 (tm_subst_tm_tm a1 x1 b) =
+      tm_subst_tm_tm a1 x1 (tm_subst_tm_tm a2 x2 b).
+Proof. intros. eapply subst_commute; auto.
+Qed.
+
+Lemma chain_subst_subst_commute : forall a p x a' b,
+      tm_pattern_agree a p ->
+      x `notin` fv_tm_tm_tm a -> x `notin` fv_tm_tm_tm p ->
+      AtomSetImpl.inter (fv_tm_tm_tm p) (fv_tm_tm_tm a') [<=] empty ->
+      chain_subst a p (tm_subst_tm_tm a' x b) =
+      tm_subst_tm_tm a' x (chain_subst a p b).
+Proof. intros. generalize dependent b. induction H; intros; simpl; eauto.
+        - simpl in H0, H1, H2. unfold chain_subst in *. simpl.
+          rewrite fold_left_app. rewrite fold_left_app. simpl.
+          rewrite subst_commute_tm. fsetdec. fsetdec. fsetdec.
+          rewrite IHtm_pattern_agree. fsetdec. fsetdec. fsetdec. auto.
+        - simpl in H0, H1, H2. unfold chain_subst in *. simpl.
+          rewrite IHtm_pattern_agree. fsetdec. fsetdec. fsetdec. auto.
+        - simpl in H0, H1, H2. unfold chain_subst in *. simpl.
+          rewrite IHtm_pattern_agree. fsetdec. fsetdec. fsetdec. auto.
+Qed.
+
+
+Theorem MatchSubst_Rename_preserve : forall p b D D' p1 b1 D1 p2 b2 D2 a a1 a2,
+   tm_pattern_agree a p -> Rename p b p1 b1 D D1 -> Rename p b p2 b2 D' D2 ->
+   (fv_tm_tm_tm a \u fv_tm_tm_tm p \u fv_tm_tm_tm b) [<=] D ->
+   (fv_tm_tm_tm a \u fv_tm_tm_tm p \u fv_tm_tm_tm b) [<=] D' ->
+   uniq_atoms_pattern p -> MatchSubst a p1 b1 a1 -> MatchSubst a p2 b2 a2 ->
+   a1 = a2.
+Proof. intros. generalize dependent p1. generalize dependent b1.
+       generalize dependent D. generalize dependent D1. generalize dependent a1.
+       generalize dependent a2. generalize dependent p2. generalize dependent b2.
+       generalize dependent D'. generalize dependent D2. generalize dependent b.
+       induction H; intros.
+         - inversion H5. inversion H0. inversion H6. inversion H1. subst. auto.
+         - unfold uniq_atoms_pattern in *. simpl in *.
+           inversion H5; subst. inversion H7; inversion H1; subst.
+           inversion H6; subst.
+           assert (L1 : tm_pattern_agree a1 p4).
+             { eapply MatchSubst_match; eauto. }
+           assert (L2 : tm_pattern_agree a1 p5).
+             { eapply MatchSubst_match; eauto. }
+           assert (L3 : pattern_renamed p1 p4 D D'0).
+             { eapply Rename_pattern_renamed; eauto. }
+           assert (L4 : pattern_renamed p1 p5 D' D'1).
+             { eapply Rename_pattern_renamed; eauto. }
+           pose (P1 := matchsubst_ind_fun H18).
+           pose (P2 := matchsubst_ind_fun H20). rewrite <- P1. rewrite <- P2.
+           rewrite matchsubst_chain_subst. auto.
+           rewrite matchsubst_chain_subst. auto.
+           pose (P3 := Rename_chain_subst H16).
+           pose (P4 := Rename_chain_subst H27). rewrite P3. rewrite P4.
+           pick fresh z.
+           assert 
+           (HYP : chain_subst a1 p4 (chain_subst p4 p1
+                      (tm_subst_tm_tm (a_Var_f z) x b)) =
+                  chain_subst a1 p5 (chain_subst p5 p1
+                      (tm_subst_tm_tm (a_Var_f z) x b))).
+           { apply IHtm_pattern_agree with (b := tm_subst_tm_tm (a_Var_f z) x b)
+             (D := D \u singleton z)(D1 := D'0)(p3 := p4)
+             (b1 := chain_subst p4 p1 (tm_subst_tm_tm (a_Var_f z) x b))
+             (D' := D' \u singleton z)(D2 := D'1)(p2 := p5)
+             (b2 := chain_subst p5 p1 (tm_subst_tm_tm (a_Var_f z) x b)).
+             unfold uniq_atoms in *.
+             eapply uniq_app_1. rewrite map_app in H4. eauto.
+             pose (R1 := fv_tm_tm_tm_tm_subst_tm_tm_upper b (a_Var_f z) x).
+             simpl in R1. apply Subset_trans with (D2 := fv_tm_tm_tm a1 \u
+             fv_tm_tm_tm p1 \u singleton z \u 
+             (Metatheory.remove x (fv_tm_tm_tm b))). eapply Subset_union.
+             eauto. eapply Subset_union. eauto. auto. fsetdec.
+           rewrite <- tm_subst_tm_tm_back_forth with (x := y) (y := z)
+          (b := tm_subst_tm_tm (a_Var_f y) x (chain_subst p4 p1 b)).
+           rewrite -> subst_via_tm with (y := y) (b := chain_subst p4 p1 b).
+           rewrite -> chain_subst_subst_commute with (a' := a_Var_f y) (x := z).
+           rewrite -> subst_via_tm with (y := y).
+           rewrite <- chain_subst_subst_commute with (a' := a_Var_f z).
+         - unfold uniq_atoms_pattern in *. simpl in *.
+           inversion H5; subst. inversion H7; inversion H1; subst.
+           inversion H6; subst.
+           eapply IHtm_pattern_agree with (b := b)(D' := D') (D := D). auto.
+           fsetdec. eapply H17. auto. fsetdec. eapply H9. auto.
+         - unfold uniq_atoms_pattern in *. simpl in *.
+           inversion H0; subst. inversion H5; inversion H1; subst.
+           inversion H6; subst.
+           eapply IHtm_pattern_agree with (b := b)(D' := D') (D := D). auto.
+           fsetdec. eapply H14. auto. fsetdec. eapply H8. auto.
+Admitted.
